\PassOptionsToPackage{naturalnames}{hyperref}
\RequirePackage{luatex85}
\documentclass{article}
\usepackage{geometry}
%\usepackage{fullpage}
\usepackage{parskip}
\usepackage{physics}
\usepackage{amsmath}
\usepackage{amssymb}
\usepackage{xcolor}
\usepackage[colorlinks,linkcolor=blue,citecolor=green]{hyperref}
\usepackage{array}
\usepackage{longtable}
\usepackage{multirow}
\usepackage{comment}
\usepackage{graphicx}
\usepackage{cite}
\usepackage{amsfonts}
\usepackage{bm}
\usepackage{slashed}
\usepackage{dsfont}
\usepackage{mathtools}
\usepackage[compat=1.1.0]{tikz-feynman}
\usepackage{simplewick}
%\usepackage{fourier}
%\usepackage{slashbox}
%\usepackage{intent}
\usepackage{mathrsfs}
\usepackage{xparse}
\usepackage{enumerate}
%\usepackage{axodraw4j}


\geometry{left=0.9cm,right=0.9cm,top=1.5cm,bottom=2cm}

\newcommand{\gm}{\gamma^{\mu}}
\newcommand{\gn}{\gamma^{\nu}}
\newcommand{\gs}{\gamma^{\sigma}}
\newcommand{\gr}{\gamma^{\rho}}
\newcommand{\gnr}{g^{\nu\rho}}
\newcommand{\gmr}{g^{\mu\rho}}
\newcommand{\gms}{g^{\mu\sigma}}
\newcommand{\gns}{g^{\nu\sigma}}
\newcommand{\vbp}{\vb{p}}
\newcommand{\vbk}{\vb{k}}
\newcommand{\g}{\gamma}
\renewcommand{\a}{\alpha}
\renewcommand{\b}{\beta}
\renewcommand{\t}{\theta}
\newcommand{\la}{\lambda}
\newcommand{\p}{\phi}
\newcommand{\vp}{\varphi}
\newcommand{\s}{\sigma}
\newcommand{\G}{\Gamma}
\newcommand{\pars}{\slashed\partial}
\newcommand{\ps}{\slashed p}
\newcommand{\ks}{\slashed k}
\newcommand{\lag}{\mathcal{L}}
\newcommand{\da}{^{\dagger}}
\newcommand{\sm}{^{\mu}}
\newcommand{\sn}{^{\nu}}
\newcommand{\smn}{^{\mu\nu}}
\newcommand{\Dm}{D^{\mu}}
\newcommand{\dm}{\partial^{\mu}}
\newcommand{\Asquare}{A^{\mu}A_{\mu}}
\newcommand{\partialsquare}[2]{\partial^{\mu}{#1}\partial_{\mu}{#2}}

\title{Hydrogen}
\author{Yingsheng Huang}
\begin{document}
\maketitle
\section{Matching}
QED Lagrangian is 
\begin{align}
  \lag_{QED}=\bar l(i\slashed D-m)l+\bar N(i D^0)N-\lag_{\gamma}
  \label{}
\end{align}
Set the NRQED Lagrangian as (take large $M$ limit where $M$ is the mass of the proton/hydrogen nucleus)
\begin{align}
  \lag_{NRQED}=\psi^{\dagger}(iD_0+\frac{\vb{D}^2}{2m})\psi+\bar N(iD_0)N+\lag_{4-fer}+\lag_{\gamma}
  \label{}
\end{align}
In tree level
\begin{align*}
  i\mathcal{M}_{QED}^{(0)}&=\feynmandiagram[horizontal=i1 to f1,layered layout,inline=($(a)!0.5!(c)$),medium]{
	i1[particle=$P_N$] -- [double distance=1pt] a -- [double distance=1pt] f1[particle=$P_N$],
	i2[particle=$p_1$] -- [fermion] c -- [fermion] f2[particle=$p_2$],
	{ [same layer] a -- [photon,momentum'=$q$] c},
  };=-e^2\bar u_N(P_N)v^{\mu}u_N(P_N)\frac{i}{\vb{q}^2}\bar u_e(p_2)\g_{\mu}u_e(p1)
\end{align*}
\begin{align*}
  i\mathcal{M}_{NRQED}^{(0)}&=\feynmandiagram[horizontal=i1 to f1,layered layout,inline=($(a)!0.5!(c)$),medium]{
	i1[particle=$P_N$] -- [double distance=1pt] a -- [double distance=1pt] f1[particle=$P_N$],
	i2[particle=$p_1$] -- [fermion] c -- [fermion] f2[particle=$p_2$],
	{ [same layer] a -- [photon,momentum'=$q$] c},
  };=-e^2\bar u_N(P_N)v^{\mu}u_N(P_N)\frac{i}{\vb{q}^2}\psi^{\dagger}(p_2)\g_{\mu}\psi(p1)
\end{align*}

The box %and crossed box 
diagram for NRQED process is
\begin{align*}
  i\mathcal{M}_{NRQED}^{(1)}&=\feynmandiagram[horizontal=i1 to f1,layered layout,inline=($(a)!0.5!(c)$),medium]{
	i1[particle=$P_N$] -- [double distance=1pt] a -- [double distance=1pt,momentum=$P_N-k$] b -- [double distance=1pt] f1[particle=$P_N$],
	i2[particle=$p_1$] -- [fermion] c -- [fermion,momentum'=$p1+k$] d -- [fermion] f2[particle=$p_2$],
	{ [same layer] a -- [photon,momentum'=$k$] c},
	{ [same layer] b-- [photon,rmomentum=$k-q$] d},
  };\\
  &=e^4\bar u_N(P_N)\frac{1+\g^0}{2}u_N(P_N)\psi^{\dagger}(p_2)\int[\dd k]\frac{1}{\vb{k}^2(\vb{k}-\vb{q})^2(-k^0+i\epsilon)(p_1^0+k^0-m-\frac{\vb{(p_1+k)}^2}{2m}+i\epsilon)}\psi(p_1)\\
  &=-ie^4\bar u_N(P_N)\frac{1+\g^0}{2}u_N(P_N)\psi^{\dagger}(p_2)\int\frac{\dd^3k}{(2\pi)^3}\frac{1}{\vb{k}^2(\vb{k}-\vb{q})^2(E_1-\frac{\vb{(p_1+k)}^2}{2m})}\psi(p_1)\\
  &=-ie^4\bar u_N(P_N)\frac{1+\g^0}{2}u_N(P_N)\psi^{\dagger}(p_2)\int\frac{\dd^3k}{(2\pi)^3}\frac{1}{(\vb{k}-\vb{p_1})^2(\vb{k}-\vb{p_2})^2(E_1-\frac{\vb{k}^2}{2m})}\psi(p_1)
\end{align*}
\clearpage 
The box and crossed box diagram for QED process is
\begin{align*}
  i\mathcal{M}_1^{(1)}&=\feynmandiagram[horizontal=i1 to f1,layered layout,inline=($(a)!0.5!(c)$),medium]{
	i1[particle=$P_N$] -- [double distance=1pt] a -- [double distance=1pt,momentum=$P_N-k$] b -- [double distance=1pt] f1[particle=$P_N$],
	i2[particle=$p_1$] -- [fermion] c -- [fermion,momentum'=$p1+k$] d -- [fermion] f2[particle=$p_2$],
	{ [same layer] a -- [photon,momentum'=$k$] c},
	{ [same layer] b-- [photon,rmomentum=$k-q$] d},
  };\\
  &=e^4\bar u_N(P_N)\frac{1+\g^0}{2}u_N(P_N)u_e^{\dagger}(p_2)\int[\dd k]\frac{(\slashed p_1+\slashed k+m)\g^0}{\vb{k}^2(\vb{k}-\vb{q})^2[(p_1+k)^2-m^2+i\epsilon](-k^0+i\epsilon)}u_e(p_1)\\
  &=e^4\bar u_N(P_N)\frac{1+\g^0}{2}u_N(P_N)u_e^{\dagger}(p_2)\int[\dd k]\frac{2p_1^0+\slashed k\g^0}{\vb{k}^2(\vb{k}-\vb{q})^2[(p_1+k)^2-m^2+i\epsilon](-k^0+i\epsilon)}u_e(p_1)\\
  &=ie^4\bar u_N(P_N)\frac{1+\g^0}{2}u_N(P_N)u_e^{\dagger}(p_2)\int\frac{\dd^3 k}{(2\pi)^3}\frac{p_1^0+k_i\g^i\g^0+\sqrt{(\vb{k}+\vb{p_1})^2+m^2}}{2\vb{k}^2(\vb{k}-\vb{q})^2[(\vb{k}+\vb{p_1})^2+m^2-p_1^0\sqrt{(\vb{k}+\vb{p_1})^2+m^2}]}u_e(p_1)\\
  &=ie^4\bar u_N(P_N)\frac{1+\g^0}{2}u_N(P_N)u_e^{\dagger}(p_2)\int\frac{\dd^3 k}{(2\pi)^3}\frac{p_1^0+(k_i-p_{1i})\g^i\g^0+\sqrt{\vb{k}^2+m^2}}{2(\vb{k}-\vb{p_1})^2(\vb{k}-\vb{p_2})^2[\vb{k}^2+m^2-p_1^0\sqrt{\vb{k}^2+m^2}]}u_e(p_1)
 \end{align*}
 $i\mathcal{M}_1^{(1)}$ has infrared log divergence and no ultraviolet divergence.
 \begin{align*}
  i\mathcal{M}_2^{(1)}&=\begin{tikzpicture}[baseline=($(a)!0.5!(c)$)]
	\begin{feynman}
	  \diagram[horizontal=i1 to f1,layered layout,medium]{
		i1[particle=$P_N$] -- [double distance=1pt] a -- [double distance=1pt,momentum=$P_N+k$] b -- [double distance=1pt] f1[particle=$P_N$],
	i2[particle=$p_1$] -- [fermion] c -- [fermion,momentum'=$p1+k$] d -- [fermion] f2[particle=$p_2$],
	{ [same layer] a --[draw=none] c},
	{ [same layer] b-- [draw=none] d},
  };
	  \diagram*{
		(a) -- [photon,rmomentum=$k-q$] (d),
		(b) -- [photon,momentum'=$k$] (c),
	  };
	\end{feynman}
  \end{tikzpicture}\\
  &=e^4\bar u_N(P_N)\frac{1+\g^0}{2}u_N(P_N)u_e^{\dagger}(p_2)\int[\dd k]\frac{(\slashed p_1+\slashed k+m)\g^0}{\vb{k}^2(\vb{k}-\vb{q})^2[(p_1+k)^2-m^2+i\epsilon](k^0+i\epsilon)}u_e(p_1)\\
  &=e^4\bar u_N(P_N)\frac{1+\g^0}{2}u_N(P_N)u_e^{\dagger}(p_2)\int[\dd k]\frac{2p_1^0+\slashed k\g^0}{\vb{k}^2(\vb{k}-\vb{q})^2[(p_1+k)^2-m^2+i\epsilon](k^0+i\epsilon)}u_e(p_1)\\
  &=-ie^4\bar u_N(P_N)\frac{1+\g^0}{2}u_N(P_N)u_e^{\dagger}(p_2)\int\frac{\dd^3 k}{(2\pi)^3}\frac{p_1^0+k_i\g^i\g^0-\sqrt{(\vb{k}+\vb{p_1})^2+m^2}}{2\vb{k}^2(\vb{k}-\vb{q})^2[(\vb{k}+\vb{p_1})^2+m^2+p_1^0\sqrt{(\vb{k}+\vb{p_1})^2+m^2}]}u_e(p_1)\\
  &=-ie^4\bar u_N(P_N)\frac{1+\g^0}{2}u_N(P_N)u_e^{\dagger}(p_2)\int\frac{\dd^3 k}{(2\pi)^3}\frac{p_1^0+(k_i-p_{1i})\g^i\g^0-\sqrt{\vb{k}^2+m^2}}{2(\vb{k}-\vb{p_1})^2(\vb{k}-\vb{p_2})^2[\vb{k}^2+m^2+p_1^0\sqrt{\vb{k}^2+m^2}]}u_e(p_1)
 \end{align*}
 $i\mathcal{M}_2^{(1)}$ has no infrared or ultraviolet divergence.
%\includegraphics[width=0.5\textwidth]{NRQED.eps}
 \begin{align*}
 i\mathcal{M}_1^{(1)}+i\mathcal{M}_2^{(1)}&=ie^4\bar u_N(P_N)\frac{1+\g^0}{2}u_N(P_N)u_e^{\dagger}(p_2)\int\frac{\dd^3 k}{(2\pi)^3}\frac{{p_1^0}^2+k^2+m^2+(k_i-p_{1i})p_1^0\g^i\g^0}{(\vb{k}-\vb{p_1})^2(\vb{k}-\vb{p_2})^2[\vb{k}^2+m^2-{p_1^0}^2]\sqrt{\vb{k}^2+m^2}}u_e(p_1)\\
 &=ie^4\bar u_N(P_N)\frac{1+\g^0}{2}u_N(P_N)u_e^{\dagger}(p_2)\int\frac{\dd^3 k}{(2\pi)^3}\frac{{p_1^0}^2+k^2+m^2+(k_i-p_{1i})p_1^0\g^i\g^0}{(\vb{k}-\vb{p_1})^2(\vb{k}-\vb{p_2})^2[\vb{k}^2-\vb{p_1}^2]\sqrt{\vb{k}^2+m^2}}u_e(p_1)
 \end{align*}
 Note that after the expansion over external momentum, $k^i$ can be converted into $p^i$ so it's actually at $p^1$ order.

 Now consider operator product expansion. 

 Tree level matching: \includegraphics[width=1.2 in]{OPE-00.eps} \& \includegraphics[width=1.2 in]{OPE-0.eps}

 \begin{align*}
   &\mel{0}{T\psi(x)N(0)}{pP_N} = \begin{tikzpicture}[baseline=($(p1)!0.5!(x)$)]
	\begin{feynman}
    \vertex (p1);
	\vertex[right=2cm of p1] (p2);
	\vertex at ($(p1)!0.4!(p2)+(0,2cm)$) (x) {$x$};
	\vertex at ($(p1)!0.6!(p2)+(0,2cm)$) (0) {$0$};
	%
	\diagram* {
      (p1) -- [momentum=\(p_{1}\), fermion] (x);
	  (p2) -- [momentum'=\(P_{N}\), double distance=1pt] (0);
    };
  \end{feynman}
\end{tikzpicture}= u_e(p)u_N(P_N)e^{-ip\cdot x}\\
   &\mel{0}{T\psi_e(x)N(0)}{pP_N} = \begin{tikzpicture}[baseline=($(p1)!0.5!(x)$)]
	\begin{feynman}
    \vertex (p1);
	\vertex[right=2cm of p1] (p2);
	\vertex at ($(p1)!0.5!(p2)+(0,2cm)$) (x);
	%
	\diagram* {
	  (p1) -- [momentum=\(p_{1}\), fermion] (x) [particle=$0$];
	  (p2) -- [momentum'=\(P_{N}\), double distance=1pt] (x);
    };
  \end{feynman}
\end{tikzpicture}=\psi_e(p)u_N(P_N)
\end{align*}
At leading order $u_e(p)=\pmqty{\psi_e(p)\\0}$.

%\begin{align*}

%\end{align*}

 One loop scenario for NRQED case:
 \includegraphics[width=1.2 in]{OPE-1.eps}
 \begin{align*}
    \mel{0}{\psi_e(0)N(0)e\int\dd^4y\bar\psi_e\psi_e A^0e\int\dd^4z\bar NNA^0}{eN}&=e^2u_N(P_N)\int[\dd k]\frac{1}{\vb{k}^2(-k^0+i\epsilon)(p_1^0+k^0-m-\frac{\vb{(p_1+k)}^2}{2m}+i\epsilon)}\psi(p_1)\\
  &=-ie^2u_N(P_N)\int\frac{\dd^3k}{(2\pi)^3}\frac{1}{\vb{k}^2(E_1-\frac{\vb{(p_1+k)}^2}{2m}+i\epsilon)}\psi(p_1)\\
  &=-ie^2u_N(P_N)\int\frac{\dd^3k}{(2\pi)^3}\frac{1}{(\vb{k}-\vb{p_1})^2(E_1-\frac{\vb{k}^2}{2m}+i\epsilon)}\psi(p_1)\\
  \intertext{drop $p_1$}
  &=-ie^2u_N(P_N)\int\frac{\dd^3k}{(2\pi)^3}\frac{1}{\vb{k}^2(E_1-\frac{\vb{k}^2}{2m}+i\epsilon)}\psi(p_1)=\pi ie^2\sqrt{\frac{2m}{E_1}}u_N(P_N)\psi(p_1)
 \end{align*}
For QED case:
\includegraphics[width=1.2 in]{OPE-2.eps}
\begin{align*}
  \mel{0}{\psi(x)N(0)e\int\dd^4y\bar\psi\g^0\psi A^0 e\int\dd^4 z \bar N NA^0}{eN}&=e^2u_N(P_N)\int[\dd k]e^{-i\vb{(k+p_1)}\cdot\vb{x}}\frac{(\slashed p_1+\slashed k+m)\g^0}{\vb{k}^2[(p_1+k)^2-m^2+i\epsilon](-k^0+i\epsilon)}u_e(p_1)\\
  &=e^2u_N(P_N)\int[\dd k]e^{-i\vb{(k+p_1)}\cdot\vb{x}}\frac{2p_1^0+\slashed k\g^0}{\vb{k}^2[(p_1+k)^2-m^2+i\epsilon](-k^0+i\epsilon)}u_e(p_1)\\
  &=ie^2u_N(P_N)\int\frac{\dd^3 k}{(2\pi)^3}e^{-i\vb{(k+p_1)}\cdot\vb{x}}\frac{p_1^0+k_i\g^i\g^0+\sqrt{(\vb{k}+\vb{p_1})^2+m^2}}{2\vb{k}^2[(\vb{k}+\vb{p_1})^2+m^2-p_1^0\sqrt{(\vb{k}+\vb{p_1})^2+m^2}]}u_e(p_1)\\
  &=ie^2u_N(P_N)\int\frac{\dd^3 k}{(2\pi)^3}e^{-i\vb{k}\cdot\vb{x}}\frac{p_1^0+(k_i-p_{1i})\g^i\g^0+\sqrt{\vb{k}^2+m^2}}{2(\vb{k}-\vb{p_1})^2[\vb{k}^2+m^2-p_1^0\sqrt{\vb{k}^2+m^2}]}u_e(p_1)\\
  \intertext{drop $p_1$}
  &=ie^2u_N(P_N)\int\frac{\dd^3 k}{(2\pi)^3}e^{-i\vb{k}\cdot\vb{x}}\frac{p_1^0+\sqrt{\vb{k}^2+m^2}}{2\vb{k}^2[\vb{k}^2+m^2-p_1^0\sqrt{\vb{k}^2+m^2}]}u_e(p_1)
 \end{align*}

 Two loop scenario for QED case $\mel{0}{T\psi(x)N(0)e\int\dd^4y_1\bar\psi\g^0\psi A^0 e\int\dd^4 z_1 \bar N NA^0e\int\dd^4y_2\bar\psi\g^0\psi A^0 e\int\dd^4 z_2 \bar N NA^0}{0}$:
 \begin{align*}
   \begin{tikzpicture}[baseline=($(p1)!0.5!(x)$)]
	\begin{feynman}
    \vertex (p1);
	\vertex[right=3cm of p1] (p2);
	\vertex at ($(p1)!0.4!(p2)+(0,3.5cm)$) (x) {$x$};
	\vertex at ($(p1)!0.6!(p2)+(0,3.5cm)$) (0) {$0$};
	\vertex at ($(p1)!0.2!(x)$) (y1);
	\vertex at ($(p2)!0.2!(0)$) (z1);
	\vertex at ($(p1)!0.6!(x)$) (y2);
	\vertex at ($(p2)!0.6!(0)$) (z2);
	%
	\diagram* {
	  (p1) -- [fermion] (x);
	  (p2) -- [double distance=1pt] (0);
	  (y1) -- [photon,rmomentum=$k_1$] (z1);
	  (y2) -- [photon,rmomentum=$k_2$] (z2);
	  (p1) -- [momentum=\(p_{1}\)] (y1);
	  (p2) -- [momentum'=\(P_{N}\),double distance=1pt] (z1);
	  (y1) -- [momentum=\(p_{1}+k_1\)] (y2);
	  (z1) -- [momentum'=\(P_{N}-k_1\),double distance=1pt] (z2);
	  (y2) -- [momentum=\(p_{1}+k_1+k_2\)] (x);
	  (z2) -- [momentum'=\(P_{N}-k_1-k_2\),double distance=1pt] (0);
    };
	\end{feynman}
  \end{tikzpicture}
  &=e^4\int[dk_1][dk_2]e^{-i\vb{(p_1+k_1+k_2)}\vdot \vb{x}}\frac{\slashed p_1+\slashed k_1+m}{}u_N(P_N)u_e(p)
 \end{align*}
 \section{HSET}
 \subsection{Lagrangian}
For scalar QED
$$\mathcal{L}=(D_{\mu}\phi)^{\dagger}D^{\mu}\phi-m^2\phi^{\dagger}\phi$$
where
$$D_{\mu}=\partial_{\mu}+ieA_{\mu}$$
In Schwartz's QFT (Chap. 35) he mentioned a choice of $\chi_v$ and $\tilde \chi_v$:
\begin{align}
\phi(x)=e^{-imv\cdot x}\frac{1}{\sqrt{2m}}(\chi_v(x)+\tilde\chi_v(x))
\label{scalar}
\end{align}
\begin{align}
\chi_v(x)=e^{imv\cdot x}\frac{1}{\sqrt{2m}}(iv\cdot D+m)\phi(x),\;
\tilde\chi_v(x)=e^{imv\cdot x}\frac{1}{\sqrt{2m}}(-iv\cdot D+m)\phi(x)
\label{scalar redefine}
\end{align}
Put \eqref{scalar} into \eqref{scalar redefine}, a simple relation is derived:
$$(-iv\cdot D)\chi_v(x)=(2m+iv\cdot D)\tilde\chi_v(x)$$
It can also be writen as 
$$2m\tilde\chi_v=(-iv\cdot D)(\chi_v+\tilde\chi_v) $$
Use this result 
\begin{align*}
  \mathcal{L}&=\frac{1}{2m}\Big\{\Bqty{[D^{\mu}(\chi_v+\tilde\chi_v)]^{\dagger}+imv^{\mu}(\chi_v+\tilde\chi_v)^{\dagger}}\Bqty{[D_{\mu}(\chi_v+\tilde\chi_v)]-imv_{\mu}(\chi_v+\tilde\chi_v)}-m^2(\chi_v+\tilde\chi_v)^{\dagger}(\chi_v+\tilde\chi_v)\Big\}\\
  &=(\chi_v+\tilde\chi_v)^{\dagger}(iv\cdot D)(\chi_v+\tilde\chi_v)+\frac{1}{2m}[D^{\mu}(\chi_v+\tilde\chi_v)]^{\dagger}D_{\mu}(\chi_v+\tilde\chi_v)
  \stepcounter{equation}\tag{\theequation}\label{lag0}\\
&=(\chi_v(x)+\tilde\chi_v(x))^{\dagger}(iv\cdot D)(\chi_v(x)+\tilde\chi_v(x))+\mathcal{O}(\frac{1}{m}) \stepcounter{equation}\tag{\theequation}\label{lag1}
\end{align*}
(note that $D_{\mu}\phi=e^{-imv\cdot x}[D_{\mu}(\chi_v+\tilde \chi_v)-imv_{\mu}(\chi_v+\tilde\chi_v)]$ and $-imv^{\mu}[D_{\mu}(\chi_v+\tilde \chi_v)]^{\dagger}(\chi_v+\tilde \chi_v)=imv^{\mu}(\chi_v+\tilde\chi_v)^{\dagger}D_{\mu}(\chi_v+\tilde \chi_v)-total\ derivative\ term$)

Use the leading order of \eqref{lag0} 
\begin{align*}
  \lag^{(0)}&=(\chi_v+\tilde\chi_v)^{\dagger}(iv\cdot D)(\chi_v+\tilde\chi_v)\\
  &=\chi_v^{\dagger}iv\cdot D\chi_v+\tilde\chi_v^{\dagger}iv\cdot D(\chi_v+\tilde\chi_v)+\chi_v^{\dagger}iv\cdot D\tilde\chi_v\\
  &=\chi_v^{\dagger}iv\cdot D\chi_v-2m\tilde\chi_v^{\dagger}\tilde\chi_v+(iv\cdot D\chi_v)^{\dagger}\tilde\chi_v\\
&=\chi_v^{\dagger}iv\cdot D\chi_v-2m\tilde\chi_v^{\dagger}\tilde\chi_v+[(-2m-iv\cdot D)\tilde\chi_v]^{\dagger}\tilde\chi_v\\
&=\chi_v^{\dagger}iv\cdot D\chi_v-\tilde\chi_v^{\dagger}(iv\cdot D+4m)\tilde\chi_v
\end{align*}

We can have the final form
$$\mathcal{L}=\chi_v^{\dagger}iv\cdot D\chi_v-\tilde \chi_v^{\dagger}(iv\cdot D+4m)\tilde\chi_v+\mathcal{O}(\frac{1}{m})$$
\subsection{Quantization}
\subsubsection{HQET as an example}
The leading term of HQET Lagrangian is 
\begin{align*}
  \lag=\bar Q_v(iv\cdot D)Q_v
\end{align*}
\begin{align*}
  Q_v(x)=e^{imv\cdot x}\frac{1+\slashed v}{2}\psi(x)
\end{align*}
In free Dirac fermion theory we know that 
\begin{align*}
    \Bqty{\psi_a(\vb{x}),\psi_b^{\dagger}(\vb{y})}=\delta^{(3)}(\vb{x}-\vb{y})\delta_{ab}\\
	\{a_{\vb{p}},a_{\vb{p'}}^{\dagger}\}=(2\pi)^3\delta^{(3)}(\vb{p-p'})
\end{align*}
also the plane wave expansion of $\psi$ is 
\begin{align*}
  \psi(x)&=\int\frac{\dd^3p}{(2\pi)^3}\frac{1}{\sqrt{2E_p}}a_{\vb{p}}u(p)e^{-ip\cdot x}\\
  &=\int \frac{\dd^3k}{(2\pi)^3}\frac{1}{\sqrt{2mv^0}}a_v\sqrt{m}u(v)e^{-imv\cdot x-ik\cdot x}\\
  \intertext{using normalization of states $u(k)=\sqrt{m}u(v)$\footnotemark, $\braket{p'}{p}=2E_p(2\pi)^3 \delta^{(3)}(\vb{p'-p})$ and $\braket{v',k'}{v,k}=2v^0\delta_{vv'}(2\pi)^3 \delta^{(3)}(\vb{k'-k})$ we have $\ket{p}=\sqrt{m}\ket{v}$ ($\ket{p}=\sqrt{2E_p}a_{\vb{p}}^{\dagger}\ket{0}$ while $\ket{v,k}=\sqrt{2v^0}a_{v,\vb{k}}^{\dagger}\ket{0}$)}
  &=\int \frac{\dd^3k}{(2\pi)^3}\frac{1}{\sqrt{2v^0}}a_vu(v)e^{-imv\cdot x-ik\cdot x}
\end{align*}
\footnotetext{The relation $\bar u^s(p)\gm u^s(p)=2p^{\mu}$ can be derived using Gordon identity, same for $\bar u^s(v)\gm u^s(v)=2v^{\mu}$, but it's actually $\bar u u$.}
Using the definition of $ Q_v(x)$
\begin{align*}
  Q_v(x)&=e^{imv\cdot x}\frac{1+\slashed v}{2}\psi(x)\\
  &=\int \frac{\dd^3k}{(2\pi)^3}\frac{1}{\sqrt{2v^0}}a_v \frac{1+\slashed v}{2}u(v)e^{-ik\cdot x}\\
  &=\int \frac{\dd^3k}{(2\pi)^3}\frac{1}{\sqrt{2v^0}}a_v u(v)e^{-ik\cdot x}
\end{align*}
The commutation relation should be 
\begin{align*}
  \{Q_{va}(\vb{x}),Q_{v'b}(\vb{x'})\}&=\int \frac{\dd^3k}{(2\pi)^3}\frac{\dd^3k'}{(2\pi)^3}\frac{1}{\sqrt{4v^0v'^0}}\{a_v,a_{v'}^{\dagger}\}u_a(v)u_b^{\dagger}(v')e^{-ik\cdot x+ik'\cdot x'}\\
  \intertext{
  using $\sum_s u_a(v)u_b^{\dagger}(v)=\frac{1}{m}\sum_s u_a(p)u^{\dagger}_b(p)=[(\slashed v+1)\g^0]_{ab}$}
  &=\int \frac{\dd^3k}{(2\pi)^3}\frac{\dd^3k'}{(2\pi)^3}\frac{1}{\sqrt{4v^0v'^0}}\{a_v,a_{v'}^{\dagger}\}[(\slashed v+1)\g^0]_{ab}e^{-ik\cdot x+ik'\cdot x'}\\
  \intertext{assuming $\{a_v,a_{v'}\}=(2\pi)^3\delta_{vv'}\delta^{(3)}(\vb{k-k'})$}
  &=\int \frac{\dd^3k}{(2\pi)^3}\frac{1}{2v^0}[(\slashed v+1)\g^0]_{ab}e^{-ik\cdot (x-x')}\delta_{vv'}\\
  &=[\frac{(\slashed v+1)\g^0}{2v^0}]_{ab}\delta_{vv'}\delta^{(3)}(\vb{x-x'})
\end{align*}
\subsubsection{HSET}
The anti-particle field is decoupled so we don't have to consider that for now. The equation-of-motion is 
\begin{align*}
  \begin{cases} 
	v\cdot D\chi_v^{\dagger}=0\\
	v\cdot D\chi_v=0
  \end{cases}
\end{align*}
By definition
\begin{align*}
  \chi_v(x)&=\frac{e^{imv\cdot x}}{\sqrt{2m}}(iv\cdot D+m)\phi(x)\\
  &=\frac{1}{\sqrt{2m}}(iv\cdot D+2m)e^{imv\cdot x}\phi(x)
\end{align*}


\end{document}


