\PassOptionsToPackage{naturalnames}{hyperref}
\RequirePackage{luatex85}
\documentclass{article}
\usepackage{geometry}
%\usepackage{fullpage}
\usepackage{parskip}
\usepackage{physics}
\usepackage{amsmath}
\usepackage{amssymb}
\usepackage{xcolor}
\usepackage[colorlinks,linkcolor=blue,citecolor=green]{hyperref}
\usepackage{array}
\usepackage{longtable}
\usepackage{multirow}
\usepackage{comment}
\usepackage{graphicx}
\usepackage{cite}
\usepackage{amsfonts}
\usepackage{bm}
\usepackage{slashed}
\usepackage{dsfont}
\usepackage{mathtools}
\usepackage[compat=1.1.0]{tikz-feynman}
\usepackage{simplewick}
%\usepackage{fourier}
%\usepackage{slashbox}
%\usepackage{intent}
\usepackage{mathrsfs}
\usepackage{xparse}
\usepackage{enumerate}
%\usepackage{axodraw4j}
\usepackage[toc,page]{appendix}
\usepackage{multicol}
\usepackage{authblk}
\usepackage[T1]{fontenc}
%\usepackage[utf8]{inputenc}

%\usepackage{luatexja-fontspec}

\geometry{left=0.9cm,right=0.9cm,top=1.5cm,bottom=2cm}

\newcommand{\gm}{\gamma^{\mu}}
\newcommand{\gn}{\gamma^{\nu}}
\newcommand{\gs}{\gamma^{\sigma}}
\newcommand{\gr}{\gamma^{\rho}}
\newcommand{\gnr}{g^{\nu\rho}}
\newcommand{\gmr}{g^{\mu\rho}}
\newcommand{\gms}{g^{\mu\sigma}}
\newcommand{\gns}{g^{\nu\sigma}}
\newcommand{\vbp}{\vb{p}}
\newcommand{\vbk}{\vb{k}}
\newcommand{\g}{\gamma}
\renewcommand{\a}{\alpha}
\renewcommand{\b}{\beta}
\renewcommand{\t}{\theta}
\newcommand{\la}{\lambda}
\newcommand{\p}{\phi}
\newcommand{\vp}{\varphi}
\newcommand{\s}{\sigma}
\newcommand{\G}{\Gamma}
\newcommand{\pars}{\slashed\partial}
\newcommand{\ps}{\slashed p}
\newcommand{\ks}{\slashed k}
\newcommand{\lag}{\mathcal{L}}
\newcommand{\da}{^{\dagger}}
\newcommand{\sm}{^{\mu}}
\newcommand{\sn}{^{\nu}}
\newcommand{\smn}{^{\mu\nu}}
\newcommand{\Dm}{D^{\mu}}
\newcommand{\dm}{\partial^{\mu}}
\newcommand{\Asquare}{A^{\mu}A_{\mu}}
\newcommand{\partialsquare}[2]{\partial^{\mu}{#1}\partial_{\mu}{#2}}

%\setmainjfont[BoldFont=FandolSong-Bold]{FandolSong-Regular}
%\setsansjfont{FandolSong-Bold}
%\setlength{\parindent}{2em}
%\linespread{1.2}
%\renewcommand\Authsep{, }

\title{Scalar QED}
\author{Yingsheng Huang and Rui Yu}

\begin{document}
\maketitle
\section{Hydrogen Wavefunction Divergence in Klein-Gordon Equation and Schr\"odinger Equation}
\subsection{The Klein-Gordon part}
The Klein-Gordon Hydrogen Equation is

\begin{align}
((i\partial_0+\frac{Z\alpha}{r})^2+\nabla^2-m^2)\Psi=0
\end{align}
 
For the bound state, the eigen value and the wave function are

\begin{align}
E&=m\frac{1}{\sqrt{1+\frac{\alpha^2 Z^2}{(\frac{1}{2}+\sqrt{\frac{1}{4}-Z^2\alpha^2})^2}}}\\
\Psi&=\frac{c}{\sqrt{4\pi}}e^{-kr}r^\lambda
\end{align}

where

\begin{align}
\lambda=-\frac{1}{2}+\sqrt{\frac{1}{4}-Z^2\alpha^2}\ \ \ \ \ \ 
c=\sqrt{\frac{(2k)^{2(1+\sqrt{\frac{1}{4}-Z^2\alpha^2})}}{\Gamma(2+2\sqrt{\frac{1}{4}-Z^2\alpha^2)})}}\ \ \ \ \ \ 
k=\frac{m}{\sqrt{1+\frac{(\frac{1}{2}+\sqrt{\frac{1}{4}-Z^2\alpha^2})^2}{\alpha^2Z^2}}}
\end{align}

c is the normaliztion factor for $\int d^3r|\Psi|^2=1$. For convenience, define

\begin{align}
\Psi '=\frac{\Psi}{2(mZ\alpha)^\frac{3}{2}}
\end{align}

Now $\Psi '$ is dimensionless and expand it in $\alpha$, we get the origin divergence comes from a term

\begin{align}
-(Z\alpha)^2\log(m r)
\end{align}

the $m$ in $\log$ could be interpreted as a subtraction point $\mu$.

\subsection{The Schr\"odinger part}

The Hamiltonian is

\begin{align}
H&=H_0+H_{int}\\
H&_0=-\frac{\nabla^2}{2m}-\frac{Z\alpha}{r},\ \ \ H_{int}=\frac{\nabla^4}{8m^3}+\frac{1}{32m^4}[-\nabla^2,[-\nabla^2,-\frac{Z\alpha}{r}]]
\end{align}

The first term of $H_{int}$ is the relativistic kinematic $v^2$ correction, the second one is the Darwin term.\\
The $H_0$ gives the radial wave functions as follows

\begin{align}
R_{n0}&=\frac{2(mZ\alpha)^\frac{3}{2}}{n^\frac{3}{2}}e^{-\frac{mZ\alpha}{n}r}F(1-n,2,\frac{2mZ\alpha r}{n}),\ \ \ E_n=-\frac{Z^2\alpha^2m}{2n^2}\\
R_{k0}&=\sqrt{\frac{2}{\pi}}(mZ\alpha)^\frac{3}{2}ke^\frac{\pi}{2k}|\Gamma(1-\frac{i}{k})|e^{-imz\alpha kr}F(1+\frac{i}{k},2,2imZ\alpha kr),\ \ \ E_k=\frac{mZ^2\alpha^2k^2}{2}
\end{align} 

Within perturbation theory,$E_1^{(1)}=<\phi|H_{int}|\phi>$, in quantum mechanics, the NLO energy correction is

\begin{align}
E_1^{(1)}=E_1Z^2\alpha^2
\end{align}

The NLO corretion of the bound state wave function is

\begin{align}
\sum_{n\neq 1}a_{n1}\phi_{n00}+\int dka_{k1}\phi_{k00}
\end{align}

with 

\begin{align}
a_{n1}=\frac{<\phi_{n00}|H_{int}|\phi_{100}>}{E_1-E_n}
\end{align}

the discrete part of $(12)$ is not divergent at $r=0$. We now focus on the integration part and seperate the relativstic kinematic term and the Darwin term. Since we are only interested in the divergent part, here we give a hard cutoff $\frac{\Lambda}{m}$ as the up-limit of the integration and a also a down-limit $\lambda$, with $\lambda>>1$ (note that the following wave function have been multiplied by $2(mZ\alpha)^\frac{3}{2}$)

\begin{align}
\Phi^{(1)}(0)_{kin}=\int_\lambda^\frac{\Lambda}{m}dk \frac{2Z^2\alpha^2k^\frac{3}{2}}{2\pi(\sqrt{1-\exp(-\frac{2 \pi}{k})})}(1-\frac{2}{1+k^2}\exp(-\frac{2\arctan(k)}{k}))e^\frac{\pi}{2k}|\Gamma(1-\frac{i}{k})|
\end{align}

with the integral region we defined$(k>>1)$, it would be OK to expand the integrand in $\frac{1}{k}$ (I havn't prove it yet), then the UV divergent term is

\begin{align}
\Phi^{(1)}(0)_{kin}&=\int_\lambda^\frac{\Lambda}{m}dk(Z\alpha)^2(\frac{1}{\pi}+\frac{1}{k})\\
&\sim(\alpha Z)^2(\frac{\Lambda}{\pi m}+\log(\frac{\Lambda}{m}))
\end{align}

The UV divergent part of Darwin term is
\begin{align}
\Phi^{(1)}(0)_D=-\frac{(Z\alpha)^4}{8\pi}\int_\lambda^\frac{\Lambda}{m}dkk^2e^\frac{\pi}{k}|\Gamma(1-\frac{i}{k})|^2
\end{align}

with the same trick as $(15)$, the UV divergen part is

\begin{align}
\Phi^{(1)}(0)_{D}&=-(\alpha Z)^4\int_\lambda^\frac{\Lambda}{m}dk\frac{k^2}{8\pi}+\frac{k}{8}+\frac{1}{24}\pi\\
&\sim -\frac{(Z\alpha)^4}{8\pi}(\frac{\Lambda^3}{3m^3}+\frac{\pi\Lambda^2}{2m^2}+\frac{\pi^2\Lambda}{3m})
\end{align}

Now collect all the results we get as follow.\\
The K-G wave function's origin UV divergence is

\begin{align}
K-G\ \ UV&:-(Z\alpha)^2\log(m r)
\end{align}

The purterbative Schr\"odinger wave function's origin UV divergence, with a k cutoff $\frac{\Lambda}{m}$, is

\begin{align}
Kin\ \  UV&:(\alpha Z)^2(\frac{\Lambda}{\pi m}+\log(\frac{\Lambda}{m}))\\
Darwin\ \  UV&:-\frac{(Z\alpha)^4}{8\pi}(\frac{\Lambda^3}{3m^3}+\frac{\pi\Lambda^2}{2m^2}+\frac{\pi^2\Lambda}{3m})
\end{align}

All the $m$, under $\Lambda$ or in a $\log$, can be interpreted as a subtraction point $\mu$.

\section{Non-relativistic Scalar QED (NRSQED) Matching}
\subsection{Feynman Rules}
\subsubsection{Scalar QED (SQED)}
Lagrangian
\begin{align}
  \lag_{SQED}=\abs{D_{\mu}\phi}^2-m^2\abs{\phi}^2+\Phi_v^*iv\cdot D\Phi_v
  \label{SQEDLAG}
\end{align}
with
\begin{align*}
  D_{\mu}\phi=\partial_{\mu}\phi+ieA_{\mu}\phi
\end{align*}
and 
\begin{align*}
  D_{\mu}\Phi_v=\partial_{\mu}\Phi-iZeA_{\mu}\Phi_v
\end{align*}
But note that no $\vb{A}$ can appear in actual calculation because here only static scalar potential exists. 
And the Feynman rules
\clearpage
\begin{multicols}{2}
  \begin{align*}
	\feynmandiagram[small,horizontal=a to b]{
	a -- [momentum=$p$] b,
    };&=\frac{i}{p^2-m^2+i\epsilon}\\
	\feynmandiagram[small,horizontal=a to o,baseline=(o.base)]{
	  a -- [momentum=$p_1$] o,
	  o -- [momentum=$p_2$] b,
	  c -- [photon] o,
	};&=-ie(p_1^{\mu}+p_2^{\mu})\\
	\feynmandiagram[small,horizontal=a to b,baseline=(o.base)]{
	  a -- [momentum'=$p_1$] o -- [momentum'=$p_2$] b,
	  c -- [photon] o,
	  d -- [photon] o,
	};&=2ie^2g^{\mu\nu}
  \end{align*}
  \begin{align*}
	\feynmandiagram[small,horizontal=a to b]{
		a -- [momentum=$mv+k$,double distance=1pt] b,
	};&=\frac{i}{v\cdot k}\\
	\feynmandiagram[small,baseline=(o.base)]{
	  a -- [double distance=1pt] o -- [double distance=1pt] b,
	  c -- [photon] o,
	};&=iZev^{\mu}\\\\\\
	\feynmandiagram[small,horizontal=a to b]{
	  a [particle=$A^0$] -- [photon,momentum=$q$] b,
	};&=\frac{i}{\vb{q}^2}
  \end{align*}
\end{multicols}
\subsubsection{NRSQED}
Using the transformation $\displaystyle\phi\rightarrow\frac{e^{-imt}}{\sqrt{2m}}\varphi$, we can have the Lagrangian
\begin{align}
  \lag_{NRSQED}=\varphi^*\pqty{iD_0+\frac{\vb{D}^2}{2m}}\varphi+\delta\lag +\Phi_v^*iv\cdot D\Phi_v
  \label{NRSQEDLAG}
\end{align}
with the same notation above. Here $\vb{D}=\nabla-ie\vb{A}$.

Feynman rules are also the same except for the scalar electron side which becomes
\begin{align*}
	\feynmandiagram[small,horizontal=a to b]{
	a -- [momentum=$p$] b,
    };=\frac{i}{E-\frac{\vb{p}^2}{2m}+i\epsilon}\;\;\;\;\;\;\;\;\;\;\;\;\;\;\;
	\feynmandiagram[small,horizontal=a to o,baseline=(o.base)]{
	  a -- [momentum=$p_1$] o,
	  o -- [momentum=$p_2$] b,
	  c [particle=$A^0$] -- [photon] o,
	};=-ie
\end{align*}
We can ignore all interacting terms involving $\vb{A}$. 

Since we need to match it to $\mathcal{O}(v^2)$ order
\begin{align}
  \delta\lag=\frac{(D_0\varphi)^*(D_0\varphi)}{2m}=\frac{\dot{\varphi}^*\dot{\varphi}}{2m}+\frac{e^2\varphi^*\varphi A_0^2}{2m}-\frac{ie}{2m}A_0(\varphi^*\dot{\varphi}-\dot{\varphi}^*\varphi)
  \label{deltaLAG}
\end{align}
and it changes the Feynman rules to\footnote{In this note, $p^0$ is the zero component of relativistic four momentum, and $E=p^0-m$. }
\begin{align*}
	\feynmandiagram[small,horizontal=a to o,baseline=(o.base)]{
	  a -- [momentum=$p_1$] o,
	  o -- [momentum=$p_2$] b,
	  c [particle=$A^0$] -- [photon] o,
	};=-ie(1+\frac{E_1+E_2}{2m})\;\;\;\;\;
	\feynmandiagram[small,horizontal=a to b,baseline=(o.base)]{
	  a -- [momentum'=$p_1$] o -- [momentum'=$p_2$] b,
	  c [particle=$A^0$] -- [photon] o,
	  d [particle=$A^0$] -- [photon] o,
	};&=\frac{ie^2}{2m}
\end{align*}<++>

Since we rescaled $\phi$ by $\frac{1}{\sqrt{2m}}$ to get $\varphi$, the in/out states are also changed. We must multiply them by $\sqrt{2p^0}$ to compensate that change. 

Another way to achieve it is to use the transform rules of heavy scalar effective theory (HSET). 

\subsection{LO}
\subsubsection{SQED}
\begin{align*}
  i\mathcal{M}_{SQED}^{(0)}&=\feynmandiagram[horizontal=i1 to f1,layered layout,inline=($(a)!0.5!(c)$),medium]{
	i1[particle=$P_N$] -- [double distance=1pt] a -- [double distance=1pt] f1[particle=$P_N$],
	i2[particle=$p_1$] -- [] c -- [] f2[particle=$p_2$],
	{ [same layer] a -- [photon,momentum'=$q$] c},
  };=-e^2v^{0}\frac{i(p_1^0+p_2^0)}{\vb{q}^2}=-e^2v^0\frac{i}{\vb{q}^2}(2m+2E_1)
\end{align*}
\subsubsection{NRSQED}
 \begin{align*}
   i\mathcal{M}_{NRSQED}^{(0)}&=\feynmandiagram[horizontal=i1 to f1,layered layout,inline=($(a)!0.5!(c)$),medium]{
	i1[particle=$P_N$] -- [double distance=1pt] a -- [double distance=1pt] f1[particle=$P_N$],
	i2[particle=$p_1$] -- [] c -- [] f2[particle=$p_2$],
	{ [same layer] a -- [photon,momentum'=$q$] c},
  };=-2\sqrt{p^0_1p^0_2}e^2v^{0}\frac{i(1+\delta)}{\vb{q}^2}=-e^2v^0\times 2p_1^0\frac{i(1+\delta)}{\vb{q}^2}
\end{align*}
which gives
\begin{align*}
  \delta=\frac{p_1^0+p_2^0}{2\sqrt{p_1^0p_2^0}i}-1\approx \frac{\vb{p}_1^4-2 \vb{p}_1^2 \vb{p}_2^2+\vb{p}_2^4}{32 m^4}
\end{align*}
The new electron-photon vertex is 
\begin{align*}
	\feynmandiagram[small,horizontal=a to o,baseline=(o.base)]{
	  a -- [momentum=$p_1$] o,
	  o -- [momentum=$p_2$] b,
	  c [particle=$A^0$] -- [photon] o,
	};&=i+i\frac{\vb{p}_1^4-2 \vb{p}_1^2 \vb{p}_2^2+\vb{p}_2^4}{32 m^4}
\end{align*}
We can write the correction interacting term corresponding to $\delta$ as 
\begin{align*}
  A_0\varphi\nabla^4\varphi^*-2A_0\nabla^2\varphi^*\nabla^2\varphi+\varphi^*A_0\nabla^4\varphi&=\varphi^*\nabla^4(A_0\varphi)-2\varphi^*\nabla^2(A_0\nabla^2\varphi)+\varphi^*A_0\nabla^4\varphi\\
  &=\varphi^*(\nabla^2[\nabla^2,A_0]-[\nabla^2,A_0]\nabla^2)\varphi\\
  &=\varphi^*[\nabla^2,[\nabla^2,A_0]]\varphi
\end{align*}
which is exactly the Darwin term in Holstein's \emph{Advanced Topics in QM} with coefficient $1/32m^4$.

\subsection{NLO}
\subsubsection{SQED}
\begin{align*}
  i\mathcal{M}_{SQED}^{(1)}&=\feynmandiagram[horizontal=i1 to f1,layered layout,inline=($(a)!0.5!(c)$),medium]{
	i1[particle=$P_N$] -- [double distance=1pt] a -- [double distance=1pt,momentum=$P_N-k^0$] b -- [double distance=1pt] f1[particle=$P_N$],
	i2[particle=$p_1$] -- [] c -- [momentum=$p_1+k$] d -- [] f2[particle=$p_2$],
	{ [same layer] a -- [photon,momentum'=$k$] c},
	{ [same layer] b -- [photon,rmomentum=$k-q$] d},
  };
  +
  \begin{tikzpicture}[baseline=($(a)!0.5!(c)$)]
	\begin{feynman}
	  \diagram[horizontal=i1 to f1,layered layout,medium]{
		i1[particle=$P_N$] -- [double distance=1pt] a -- [double distance=1pt,momentum=$P_N+k$] b -- [double distance=1pt] f1[particle=$P_N$],
	i2[particle=$p_1$] -- [] c -- [momentum'=$p1+k$] d -- [] f2[particle=$p_2$],
	{ [same layer] a --[draw=none] c},
	{ [same layer] b-- [draw=none] d},
  };
	  \diagram*{
		(a) -- [photon,rmomentum=$k-q$] (d),
		(b) -- [photon,momentum'=$k$] (c),
	  };
	\end{feynman}
  \end{tikzpicture}
  +
  \begin{tikzpicture}[baseline=($(a)!0.5!(c)$)]
	\begin{feynman}
	  \diagram[horizontal=i1 to f1,layered layout,medium]{
		i1[particle=$P_N$] -- [double distance=1pt] a -- [double distance=1pt,momentum=$P_N+k$] b -- [double distance=1pt] f1[particle=$P_N$],
		i2[particle=$p_1$] -- [] c -- [] d -- [] f2[particle=$p_2$],
		{ [same layer] a --[draw=none] c},
		{ [same layer] b-- [draw=none] d},
	  };
	  \vertex at ($(c)!0.5!(d)$) (f);
	  \diagram*{
		(a) -- [photon,momentum'=$k$] (f),
		(b) -- [photon,rmomentum=$k$] (f),
	  };
	\end{feynman}
  \end{tikzpicture}
\end{align*}
\begin{align*}
  \feynmandiagram[horizontal=i1 to f1,layered layout,inline=($(a)!0.5!(c)$),medium]{
	i1[particle=$P_N$] -- [double distance=1pt] a -- [double distance=1pt,momentum=$P_N-k^0$] b -- [double distance=1pt] f1[particle=$P_N$],
	i2[particle=$p_1$] -- [] c -- [momentum=$p_1+k$] d -- [] f2[particle=$p_2$],
	{ [same layer] a -- [photon,momentum'=$k$] c},
	{ [same layer] b -- [photon,rmomentum=$k-q$] d},
  };=-e^2v^{0}\int\frac{\dd^4k}{(2\pi)^4}\frac{i}{\vb{k}^2}\frac{}{}<+content+>
\end{align*}<++>
\begin{align*}
  \begin{tikzpicture}[baseline=($(a)!0.5!(c)$)]
	\begin{feynman}
	  \diagram[horizontal=i1 to f1,layered layout,medium]{
		i1[particle=$P_N$] -- [double distance=1pt] a -- [double distance=1pt,momentum=$P_N+k$] b -- [double distance=1pt] f1[particle=$P_N$],
	i2[particle=$p_1$] -- [] c -- [momentum'=$p1+k$] d -- [] f2[particle=$p_2$],
	{ [same layer] a --[draw=none] c},
	{ [same layer] b-- [draw=none] d},
  };
	  \diagram*{
		(a) -- [photon,rmomentum=$k-q$] (d),
		(b) -- [photon,momentum'=$k$] (c),
	  };
	\end{feynman}
  \end{tikzpicture} <+content+>
\end{align*}<++>
\begin{align*}
  \begin{tikzpicture}[baseline=($(a)!0.5!(c)$)]
	\begin{feynman}
	  \diagram[horizontal=i1 to f1,layered layout,medium]{
		i1[particle=$P_N$] -- [double distance=1pt] a -- [double distance=1pt,momentum=$P_N+k$] b -- [double distance=1pt] f1[particle=$P_N$],
		i2[particle=$p_1$] -- [] c -- [] d -- [] f2[particle=$p_2$],
		{ [same layer] a --[draw=none] c},
		{ [same layer] b-- [draw=none] d},
	  };
	  \vertex at ($(c)!0.5!(d)$) (f);
	  \diagram*{
		(a) -- [photon,momentum'=$k$] (f),
		(b) -- [photon,rmomentum=$k$] (f),
	  };
	\end{feynman}
  \end{tikzpicture}<+content+>
\end{align*}<++>
\subsubsection{NRSQED}

\section{Local Operator and Matrix Element of NRSQED}
To reproduce the singular behavior of ``Klein-Gordon Hydrogen'' wavefunction near origin, we can try OPE. But the dependence of x in OPE can be taken as a regularization scheme and thus the result should be the same as local one without renormalization. And the logarithmic terms of x in OPE can be reproduced by the logarithmic divergence of local operators. Since in the study of Klein-Gordon equation we know that the wavefunction only contains logarithmic divergence at the origin so that's the only type of divergence we're looking for. 
\subsection{LO}

\subsection{NLO}
\begin{align*}
  &\mel{0}{\psi_e(0)N(0)(-ie\mu^{-\epsilon})\int\dd^4y\bar\psi_e\psi_e A^0(-ie\mu^{-\epsilon})\int\dd^4z\bar NNA^0}{eN}=\begin{tikzpicture}[baseline=($(p1)!0.5!(x)$)]
	\begin{feynman}
    \vertex (p1);
	\vertex[right=2.5cm of p1] (p2);
	\vertex at ($(p1)!0.5!(p2)+(0,2.5cm)$) (x) ;
	\vertex at ($(p1)!0.3!(x)$) (y1);
	\vertex at ($(p2)!0.3!(x)$) (z1);
	%
	\diagram* {
	  (p1) -- [] (x);
	  (p2) -- [double distance=1pt] (x);
	  (y1) -- [photon,rmomentum=$k_1$] (z1);
	  (p1) -- [momentum=\(p\)] (y1);
	  (p2) -- [momentum'=$P_{N}\text{=}m_{N}v_{N}$,double distance=1pt] (z1);
	  (y1) -- [momentum=\(p+k\)] (x);
	  (z1) -- [momentum'=\(P_{N}-k\),double distance=1pt] (x);
    };
	\end{feynman}
  \end{tikzpicture}
\end{align*}
which doesn't have logarithm divergence\footnote{After dimensional regularization, the Gamma function in the numerator is something like $\Gamma(n-d/2)$ and Gamma function doesn't have pole at half integer. We can rigorously prove this kind of diagrams do not have logarithmic divergence at one loop. }. 
\subsection{NNLO}
\begin{align*}
  &\begin{tikzpicture}[baseline=($(p1)!0.5!(x)$)]
 \begin{feynman}
   \vertex (p1);
 \vertex[right=3cm of p1] (p2);
 \vertex at ($(p1)!0.5!(p2)+(0,3.5cm)$) (x) ;
 \vertex at ($(p1)!0.2!(x)$) (y1);
 \vertex at ($(p2)!0.2!(x)$) (z1);
 \vertex at ($(p1)!0.6!(x)$) (y2);
 \vertex at ($(p2)!0.6!(x)$) (z2);
 %
 \diagram* {
   (p1) -- [] (x);
   (p2) -- [double distance=1pt] (x);
   (y1) -- [photon,rmomentum=$k_1$] (z1);
   (y2) -- [photon,rmomentum=$k_2$] (z2);
   (p1) -- [momentum=\(p\)] (y1);
   (p2) -- [momentum'=$P_{N}\text{=}m_{N}v_{N}$,double distance=1pt] (z1);
   (y1) -- [momentum=\(p+k_1\)] (y2);
   (z1) -- [momentum'=\(P_{N}-k_1\),double distance=1pt] (z2);
   (y2) -- [momentum=\(p+k_1+k_2\)] (x);
   (z2) -- [momentum'=\(P_{N}-k_1-k_2\),double distance=1pt] (x);
   };
 \end{feynman}
 \end{tikzpicture}\\ =&-\mu^{2\epsilon}Z^2e^4\bqty{\int[dk_1][dk_2]\frac{1}{\vb{\abs{k_1}}^2}\frac{1}{\vb{\abs{k_2}}^2}\frac{1}{-k_1^0-k_2^0+i\epsilon}\frac{1}{-k_1^0+i\epsilon}\frac{1}{p^0+k_1^0-m-\frac{\vb{(p+k_1)}^2}{2m}+i\epsilon}\frac{1}{p^0+k_1^0+k_2^0-m-\frac{\vb{(p+k_1+k_2)}^2}{2m}+i\epsilon}}
 \\
 \intertext{do the shift as above}
 =&\mu^{2\epsilon}Z^2e^4\bqty{\int\frac{\dd^3\vb{k_1}}{(2\pi)^3}\frac{\dd^3\vb{k_2}}{(2\pi)^3}\frac{1}{\vb{\abs{k_1-p}}^2}\frac{1}{\vb{\abs{k_2-k_1}}^2}\frac{1}{E-\frac{\vb{\abs{k_1}}^2}{2m}+2i\epsilon}\frac{1}{E-\frac{\vb{\abs{k_2}}^2}{2m}+2i\epsilon}}=0
\end{align*}
\begin{align*}
  &\begin{tikzpicture}[baseline=($(p1)!0.5!(x)$)]
 \begin{feynman}
   \vertex (p1);
 \vertex[right=3cm of p1] (p2);
 \vertex at ($(p1)!0.5!(p2)+(0,3.5cm)$) (x) ;
 \vertex at ($(p1)!0.2!(x)$) (y1);
 \vertex at ($(p2)!0.2!(x)$) (z1);
 \vertex at ($(p1)!0.6!(x)$) (y2);
 \vertex at ($(p2)!0.6!(x)$) (z2);
 \vertex at ($(y1)!0.5!(z1)$) (t);
 %
 \diagram* {
   (p1) -- [] (x);
   (p2) -- [double distance=1pt] (x);
   (y1) -- [photon,rmomentum=$k_1$] (z1);
   (y2) -- [photon,rmomentum=$k_2$] (z2);
   (p1) -- [momentum=\(p\)] (y1);
   (p2) -- [momentum'=$P_{N}\text{=}m_{N}v_{N}$,double distance=1pt] (z1);
   (y1) -- [momentum=\(p+k_1\),insertion=0.5] (y2);
   (z1) -- [momentum'=\(P_{N}-k_1\),double distance=1pt] (z2);
   (y2) -- [momentum=\(p+k_1+k_2\)] (x);
   (z2) -- [momentum'=\(P_{N}-k_1-k_2\),double distance=1pt] (x);
   };
 \end{feynman}
 \end{tikzpicture}=4m^2\mu^{2\epsilon}Z^2e^4
 \int\frac{\dd^3\vb{k_1}}{(2\pi)^3}\frac{\dd^3\vb{k_2}}{(2\pi)^3}\frac{1}{\vb{\abs{k_1-p}}^2}\frac{1}{\vb{\abs{k_2-k_1}}^2}\frac{\vb{\abs{k_1}}^4/4m^2}{[\vb{\abs{k_1}}^2-2mE]^2}\frac{1}{\vb{\abs{k_2}}^2-2mE}\\
  =&Z^2\a^2(\frac{1}{2(3-d)}+\log \mu)+\text{finite terms}
\end{align*}
\begin{align*}
  &\begin{tikzpicture}[baseline=($(p1)!0.5!(x)$)]
 \begin{feynman}
   \vertex (p1);
 \vertex[right=3cm of p1] (p2);
 \vertex at ($(p1)!0.5!(p2)+(0,3.5cm)$) (x) ;
 \vertex at ($(p1)!0.2!(x)$) (y1);
 \vertex at ($(p2)!0.2!(x)$) (z1);
 \vertex at ($(p1)!0.6!(x)$) (y2);
 \vertex at ($(p2)!0.6!(x)$) (z2);
 \vertex at ($(y1)!0.5!(z1)$) (t);
 %
 \diagram* {
   (p1) -- [] (x);
   (p2) -- [double distance=1pt] (x);
   (y1) -- [photon,rmomentum=$k_1$] (z1);
   (y2) -- [photon,rmomentum=$k_2$] (z2);
   (p1) -- [momentum=\(p\)] (y1);
   (p2) -- [momentum'=$P_{N}\text{=}m_{N}v_{N}$,double distance=1pt] (z1);
   (y1) -- [momentum=\(p+k_1\)] (y2);
   (z1) -- [momentum'=\(P_{N}-k_1\),double distance=1pt] (z2);
   (y2) -- [momentum=\(p+k_1+k_2\),insertion=0.5] (x);
   (z2) -- [momentum'=\(P_{N}-k_1-k_2\),double distance=1pt] (x);
   };
 \end{feynman}
 \end{tikzpicture}=4m^2
   \mu^{2\epsilon}Z^2e^4\int\frac{\dd^3\vb{k_1}}{(2\pi)^3}\frac{\dd^3\vb{k_2}}{(2\pi)^3}\frac{1}{\vb{\abs{k_1-p}}^2}\frac{1}{\vb{\abs{k_2-k_1}}^2}\frac{1}{\vb{\abs{k_1}}^2-2mE}\frac{\vb{\abs{k_2}}^4/4m^2}{[\vb{\abs{k_2}}^2-2mE]^2}\\
 =&0+\text{finite terms}
\end{align*}

\clearpage

\begin{appendices}
  \section{Useful formulas in Feynman integrals}
  Feynman parametrization used here is
  \begin{align}
	\frac{1}{\prod A_i^{d_i}}=\int\prod \dd x_i \delta(\sum x_i-1)\frac{\prod x_i^{d_i-1}}{\bqty{\sum x_iA_i}^{\sum d_i}}\frac{\Gamma(\sum d_i)}{\prod\Gamma(d_i)}
	\label{FEYNMANPARA}
  \end{align}
  Integral with the structure of the form 
  \begin{align*}
	\int[dk_1][dk_2]\frac{1}{\vb{\abs{k_1}}^2}\frac{1}{\vb{\abs{k_2}}^2}\frac{1}{-k_1^0-k_2^0+i\epsilon}\frac{1}{-k_1^0+i\epsilon}\frac{1}{[p^0+k_1^0-M-\frac{\vb{(p+k_1)}^2}{2M}+i\epsilon]^m}\frac{1}{[p^0+k_1^0+k_2^0-M-\frac{\vb{(p+k_1+k_2)}^2}{2M}+i\epsilon]^n}
  \end{align*}
  will always produce
  \begin{align*}
	\int\frac{\dd^3\vb{k_1}}{(2\pi)^3}\frac{\dd^3\vb{k_2}}{(2\pi)^3}\frac{1}{\vb{\abs{k_1}}^2}\frac{1}{\vb{\abs{k_2}}^2}\frac{1}{[p^0-M-\frac{\vb{(p+k_1)}^2}{2M}]^m}\frac{1}{[p^0-M-\frac{\vb{(p+k_1+k_2)}^2}{2M}+i\epsilon]^n}
  \end{align*}
  with $k_1^0$ and $k_2^0$ goes to zero.

  For arbitary one loop diagram of the following form, we have
  \begin{subequations} \label{1loopgamma}
	\begin{align}
	  \int\frac{\dd^dk}{(2\pi)^d}\frac{k^{2\b}}{(k^2+\Delta)^n}&=\frac{1}{(4\pi)^{n-\b}}\frac{\Gamma(\b+d/2)}{\Gamma(d/2)}\frac{\Gamma(n-\b-d/2)}{\Gamma(n)}\pqty{\frac{4\pi}{\Delta}}^{n-\b-d/2}\\
	  &=\frac{1}{(4\pi)^{d/2}}\frac{\Gamma(\b+d/2)}{\Gamma(d/2)}\frac{\Gamma(n-\b-d/2)}{\Gamma(n)}\pqty{\frac{1}{\Delta}}^{n-\b-d/2}
	\end{align}
  \end{subequations}
  where $\frac{1}{(4\pi)^{d/2}}$ often appears as $2^{-d}\pi^{-d/2}$.
%  For two loop diagrams of this form ($\epsilon=3-d$)
%  \begin{align}
%	\mu^{-4\epsilon}\int\frac{\dd^d\vb{k}_1}{(2\pi)^d}\frac{\dd^d\vb{k}_2}{(2\pi)^d}\frac{1}{\vb{(k_1-a)}^2}\frac{1}{\vb{(k_2-k_1)}^2}\frac{\vbk_1^{2\a}}{(\vb{k}_1^2-c)^m}\frac{\vbk_2^{2\b}}{(\vb{k}_2^2-d)^n}
%	\label{int}
%  \end{align}
%  The integral is evaluated to
%  \begin{align*}
%	&\mu^{-4\epsilon}\int_0^1\prod_{i=1}^2\dd x_i\delta(\sum x_i-1)\prod x_i^{d_i-1}\frac{\Gamma(n+1)}{\Gamma(n)}\frac{1}{(4\pi)^{n+1-\b}}\frac{\Gamma(\b+d/2)}{\Gamma(d/2)}\frac{\Gamma(n+1-\b-d/2)}{\Gamma(n+1)}\pqty{\frac{4\pi}{\a(x_i)}}^{n+1-\b-d/2}
%	\\&\int\frac{\dd^d\vb{k}_1}{(2\pi)^d}\frac{1}{\vb{(k_1-a)}^2}\frac{\vbk_1^{2\a}}{(\vb{k}_1^2-c)^m}\frac{1}{(\vb{k}_1-\Delta_2)^{n+1-\b-d/2}}\\
%	=&\mu^{-4\epsilon}\int_0^1\prod_{i=1}^2\dd x_i\delta(\sum x_i-1)\prod x_i^{d_i-1}\frac{1}{(4\pi)^{n+1-\b}}\frac{\Gamma(\b+d/2)}{\Gamma(d/2)}\frac{\Gamma(n+1-\b-d/2)}{\Gamma(n)}\pqty{\frac{4\pi}{\a(x_i)}}^{n+1-\b-d/2}\int_0^1\prod_{i=1}^3\dd y_j\delta(\sum y_j-1)
%	\\&\prod y_j^{d_j-1}
%	\frac{\Gamma(m+n+2-\b-d/2)}{\Gamma(m)\Gamma(n+1-\b-d/2)}\frac{1}{(4\pi)^{m+n+2-\a-\b-d/2}}\frac{\Gamma(\a+d/2)}{\Gamma(d/2)}\frac{\Gamma(m+n+2-\a-\b-d)}{\Gamma(m+n+2-\b-d/2)}\pqty{\frac{4\pi}{\Delta_1}}^{m+n+2-\a-\b-d}
%	\\
%	=&\mu^{-4\epsilon}\int_0^1\prod_{i=1}^2\dd x_i\delta(\sum x_i-1)\prod x_i^{d_i-1}\frac{1}{(4\pi)^{d}}\frac{\Gamma(\b+d/2)}{\Gamma(d/2)}\frac{1}{\Gamma(n)}\pqty{\frac{1}{\a(x_i)}}^{n+1-\b-d/2}
%	\\&\int_0^1\prod_{i=1}^3\dd y_j\delta(\sum y_j-1)\prod y_j^{d_j-1}\frac{\Gamma(\a+d/2)}{\Gamma(d/2)}\frac{\Gamma(m+n+2-\a-\b-d)}{\Gamma(m)}\pqty{\frac{1}{\Delta_1}}^{m+n+2-\a-\b-d}
 % \end{align*}<++>
  \section{<++>}<++>
\end{appendices}

\end{document}
