%!mode::"Tex:UTF-8"
\PassOptionsToPackage{unicode}{hyperref}
\PassOptionsToPackage{naturalnames}{hyperref}
\documentclass{article}
\usepackage{geometry}
%\usepackage{fullpage}
\usepackage{parskip}
\usepackage{physics}
\usepackage{amsmath}
\usepackage{amssymb}
\usepackage{xcolor}
\usepackage[colorlinks,linkcolor=blue,citecolor=green]{hyperref}
\usepackage{array}
\usepackage{longtable}
\usepackage{multirow}
\usepackage{comment}
\usepackage{graphicx}
\usepackage{cite}
\usepackage{amsfonts}
\usepackage{bm}
\usepackage{slashed}
\usepackage{dsfont}
\usepackage{mathtools}
\usepackage[compat=1.1.0]{tikz-feynman}
\usepackage{simplewick}
%\usepackage{fourier}
%\usepackage{slashbox}
%\usepackage{intent}
\usepackage{mathrsfs}
\usepackage{xparse}
\usepackage{enumerate}

\geometry{left=1.5cm,right=1.5cm,top=1.5cm,bottom=2cm}

\newcommand{\gm}{\gamma^{\mu}}
\newcommand{\gn}{\gamma^{\nu}}
\newcommand{\gs}{\gamma^{\sigma}}
\newcommand{\gr}{\gamma^{\rho}}
\newcommand{\gnr}{g^{\nu\rho}}
\newcommand{\gmr}{g^{\mu\rho}}
\newcommand{\gms}{g^{\mu\sigma}}
\newcommand{\gns}{g^{\nu\sigma}}
\newcommand{\vbp}{\vb{p}}
\newcommand{\vbk}{\vb{k}}
\newcommand{\g}{\gamma}
\renewcommand{\a}{\alpha}
\renewcommand{\b}{\beta}
\renewcommand{\t}{\theta}
\newcommand{\la}{\lambda}
\newcommand{\p}{\phi}
\newcommand{\vp}{\varphi}
\newcommand{\s}{\sigma}
\renewcommand{\G}{\Gamma}
\newcommand{\pars}{\slashed\partial}
\newcommand{\ps}{\slashed p}
\newcommand{\ks}{\slashed k}
\renewcommand{\L}{\Lambda}
\newcommand{\lag}{\mathcal{L}}

\title{Quantum Field Theory(Spring)}
\author{Yingsheng Huang}
\begin{document}
\maketitle
\section{Noether's Theorem}
\begin{itemize}
  \item Symmetry
  \item Lorentz/Poincare Group
  \item Tensor analysis
\end{itemize}
Poincare group: 
$$x'^{\mu}=\L^{\mu}_{\nu}x^{\nu}+a^{\mu}$$
investigate the inverse, closure character:
$$x''^{\mu}=\bar\L^{\mu}_{\rho}x'^{\rho}+\bar a^{\mu}=(\bar \L\L)^{\mu}_{\nu}x^{\nu}+(\bar \L^{\mu}_{\rho}a^{\rho}+\bar a^{\mu})$$
$$(\bar \L,\bar a)\times(\L,a)=(\bar \L\L,\bar\L a+\bar a)$$
$$x'^{\mu}=x^{\mu}+\delta x^{\mu}$$
translation:
$$\L^{\mu}_{\nu}=\delta^{\mu}_{\nu}+\omega^{\mu}_{\nu}$$
\begin{align*}
  g_{\rho\s}&=g_{\mu\nu}\L^{\mu}_{\rho}\L^{\nu}_{\s}=g_{\mu\nu}(\delta^{\mu}_{\nu''}+\omega^{\mu}_{\nu''})(\delta^{\nu}_{\nu'}+\omega^{\nu}_{\nu'}) \\
  \delta x^{\mu}&=\omega^{\mu}_{\nu}x^{\nu}\\
  &=\omega^{\mu\nu}x_{\nu}=\omega^{\rho\s}x_{\s}\delta^{\mu}_{\rho}=\omega^{\rho\s}x_{\s}\partial_{\rho}x^{\mu}\\
  &=\frac{i}{2}\omega^{\rho\s}\hat L_{\rho\s}x^{\mu}
\end{align*}
$$\hat L_{\mu\nu}=i(x_{\mu}\partial_{\nu}-x_{\nu}\partial_{\mu})$$
Poincare algebra: commutation relations.

Local field transform under Poincare group:
$$f(x)\rightarrow f'(x')$$
\begin{align*}
  \delta f\equiv f'(x')-f(x)&=f'(x+\delta x)-f(x)\\
  f'(x)-f(x)+\delta x^{\mu}\partial_{\mu}f(x)+\mathcal(O)(\delta x)\\
  &=\delta_0f+\delta x^{\mu}\partial_{\mu}
\end{align*}
$$\delta\equiv\delta_0(\text{functional change})+\delta x^{\mu}\partial_{\mu}$$
translation: 
$$\delta f=0=\delta_0f+\epsilon^{\mu}\partial_{\mu}f\Longrightarrow\delta_0f=-\epsilon^{\mu}\partial_{\mu}f=-i\epsilon\cdot\hat pf$$
Lorentz:
$$\delta_0\phi=-\delta x^{\mu}\partial_{\mu}\phi=\omega^{\mu\rho}x_{\rho}\partial_{\mu}\phi=\frac{1}{2}\omega^{\rho\s}(x_{\rho}\partial_{\s}-x_{\s}\partial_{\rho})$$
$$\delta_0\phi=-\frac{i}{2}\omega^{\rho\s}L_{\rho\s}\phi$$
$$\delta_0(\partial_{\mu}\phi)=-\frac{i}{2}\omega^{\rho\s}L_{\rho\s}(\partial_{\mu\phi})=\frac{i}{2}\omega^{\rho\s}S_{\rho\s}$$
$$\Longrightarrow(S_{\mu\nu})^{\rho}_{\s}=\dots$$

Noether's theorem:
$$\delta S=\delta\int\dd^4x\lag=\int(\delta\dd^4x)\lag+\int\dd^4x\delta\lag$$
$$\delta\dd^4x=\dd^4x(\partial_{\mu}\delta x^{\mu})$$
\begin{align*}
  \delta S&=\int\dd^4x[\partial_{\mu}(\lag\delta x)+\delta_0\lag]\\
  &=\int\dd^4x[\partial_{\mu}(\lag\delta x^{\mu})+\partial_{\mu}\dv{\lag}{(\partial_{\mu}\phi)}+\text{E-L eq terms}]\\
  &=\int_R\partial_{\mu}[\lag\delta^{\mu}_{\rho}-\dv{\lag}{(\partial_{\mu}\phi)}\partial_{\rho}\phi)\delta x^{\rho}+\dv{\lag}{(\partial_{\mu}\phi)}\delta \phi]
\end{align*}




\end{document}
